deps/poulet4/lib/P4automata/FirstOrderConfRel.v
@@ -117,4 +117,3 @@ Section AutModel.
     FirstOrder.mod_rels := mod_rels;
   |}.
 End AutModel.
-
